A bunch of updates that I lose track of

src-lite/wl_transfer.v
@@ -1,5 +1,7 @@
 Require Import worklist.
 Require Import decl_worklist.
+Require simplified_ind.
+
 
 Inductive kind_iso : kind → akind → Prop :=
 | kiso_star : kind_iso k_star ak_star
@@ -56,10 +58,10 @@ Inductive work_iso : dwork → work → Prop :=
   , expr_iso e1 e1' → expr_iso e2 e2'
   → (forall x, x `notin` L → worklist_iso (c $ `x) (c' $′ `′x))
   → work_iso (e1 <: e2 ⇒ c) (e1' <: e2' ⇒′ c')
-| wiso_iapp : forall L A A' e1 e1' e2 e2' c c'
-  , expr_iso A A' → expr_iso e1 e1' → expr_iso e2 e2'
+| wiso_iapp : forall L A A' e e1' e2' c c'
+  , expr_iso A A' → expr_iso e e1' → expr_iso e e2'
   → (forall x, x `notin` L → worklist_iso (c $ `x) (c' $′ `′x))
-  → work_iso (A ⋅ e1 & e2 ⇒ c) (A' ⋅ e1' & e2' ⇒′ c')
+  → work_iso (A ⋅ e ⇒ c) (A' ⋅ e1' & e2' ⇒′ c')
 | wiso_reduce : forall L A A' c c'
   , expr_iso A A'
   → (forall x, x `notin` L → worklist_iso (c $ `x) (c' $′ `′x))
@@ -74,6 +76,8 @@ with worklist_iso : dworklist → worklist → Prop :=
   → worklist_iso (Γ ,' x : A) (Γ' ,′ x :′ A')
 .
 
+#[export]
+Hint Constructors work_iso worklist_iso obind_iso expr_iso kind_iso : core.
 
 Reserved Notation "wl ⟿ dwl" (at level 65, no associativity).
 Inductive transfer : worklist → dworklist → Prop :=
@@ -89,3 +93,336 @@ Inductive transfer : worklist → dworklist → Prop :=
   → Γ1' ,′ ⧼^x⧽ ⫢′             Γ2' ⟿ Γ
 where "wl ⟿ dwl" := (transfer wl dwl)
 .
+
+#[export]
+Hint Constructors transfer : core.
+
+Inductive ss_entry :=
+| sse_v (A : expr)
+| sse_ex (A : expr) (e : expr)
+| sse_kv (k : kind)
+.
+
+Inductive lc_sse : ss_entry → Prop :=
+| lc_sse_v : forall A, lc_expr A → lc_sse (sse_v A)
+| lc_sse_ex : forall A e, lc_expr A → lc_expr e → lc_sse (sse_ex A e)
+| lc_sse_kv : forall k, lc_sse (sse_kv k)
+.
+
+Definition subst_set := list (var * ss_entry).
+
+Notation ": A !" :=
+  (sse_v A) (at level 52, A at level 50, no associativity).
+
+Notation ": A ≔ e" :=
+  (sse_ex A e) (at level 52, A at level 50, no associativity).
+Notation " ≔ ⧼ k ⧽" :=
+  (sse_kv k) (at level 52, no associativity).
+
+Declare Scope subst_set_scope.
+Delimit Scope subst_set_scope with subst.
+Bind Scope subst_set_scope with subst_set.
+
+Notation "s1 ;; s2" := (app s2 s1)
+  (at level 58, left associativity) : subst_set_scope.
+
+Notation "s ; x e" := (cons (pair x e) s)
+  ( at level 58, x at level 0, e at level 52, left associativity) : subst_set_scope.
+
+Notation "x e ∈ s" := (binds x e s)
+  (at level 65, e at level 52, no associativity) : type_scope.
+
+Open Scope subst_set_scope.
+
+
+(* 'ss' is short for 'substitution set' *)
+Fixpoint ss_to_ctx (s : subst_set) : context :=
+  match s with
+  | nil => ctx_nil
+  | s' ; x : A ! => ss_to_ctx s' , x : A
+  | s' ; x : A ≔ e => ss_to_ctx s'
+  | s' ; x ≔ ⧼k⧽ => ss_to_ctx s'
+  end
+.
+
+(* syntactic well-formedness of substitution set *)
+Inductive wf_ss : subst_set → Prop :=
+| wf_ss_nil : wf_ss nil
+| wf_ss_v  : forall x A Θ
+  , wf_ss Θ → x `notin` dom Θ → lc_expr A
+  → wf_ss (Θ; x : A !)
+| wf_ss_kv : forall x k Θ
+  , wf_ss Θ → x `notin` dom Θ
+  → wf_ss (Θ; x ≔ ⧼k⧽)
+| wf_ss_ex : forall x A e Θ
+  , wf_ss Θ
+  → x `notin` dom Θ → mono_type e
+  → wf_ss (Θ; x : A ≔ e)
+.
+
+Lemma wf_lc_sse : forall Θ x e,
+  binds x e Θ → wf_ss Θ → lc_sse e.
+Proof.
+Admitted.
+
+(* 'inst' is short for 'instantiate' *)
+Reserved Notation "T ⊩ e1 ⇝ e2" (at level 65, e1 at level 58, no associativity).
+Inductive inst_expr : subst_set → aexpr → expr → Prop :=
+| inste_var : forall Θ x,     wf_ss Θ → inst_expr Θ `′x `x
+| inste_ex  : forall Θ x A e, wf_ss Θ → x : A ≔ e ∈ Θ → inst_expr Θ  `^x  e
+| inste_k   : forall Θ x k,   wf_ss Θ → x ≔ ⧼k⧽ ∈ Θ → inst_expr Θ ⧼`^x⧽ ⧼k⧽
+| inste_num : forall Θ n,     wf_ss Θ → inst_expr Θ (ae_num n) (e_num n)
+| inste_int : forall Θ,       wf_ss Θ → inst_expr Θ ae_int e_int
+| inste_bot : forall Θ A' A,
+    inst_expr Θ A' A → inst_expr Θ (ae_bot A') (e_bot A)
+| inste_app : forall Θ f' f a' a
+  , inst_expr Θ f' f → inst_expr Θ a' a
+  → inst_expr Θ (ae_app f' a') (e_app f a)
+| inste_castup : forall Θ A' A e' e
+  , inst_expr Θ A' A → inst_expr Θ e' e
+  → inst_expr Θ (ae_castup A' e') (e_castup A e)
+| inste_castdn : forall Θ e' e,
+    inst_expr Θ e' e → inst_expr Θ (ae_castdn e') (e_castdn e)
+| inste_abs : forall L Θ A' A e' e B' B
+  , inst_expr Θ A' A
+  → (forall x, x `notin` L → inst_expr Θ (e' ^`′ x) (e ^` x))
+  → (forall x, x `notin` L → inst_expr Θ (B' ^`′ x) (B ^` x))
+  → inst_expr Θ (λ′ A', e' : B') (λ_ A, e : B)
+| inste_bind : forall L Θ A' A e' e B' B
+  , inst_expr Θ A' A
+  → (forall x, x `notin` L → inst_expr Θ (e' ^`′ x) (e ^` x))
+  → (forall x, x `notin` L → inst_expr Θ (B' ^`′ x) (B ^` x))
+  → inst_expr Θ (Λ′ A', e' : B') (Λ A, e : B)
+| inste_pi : forall L Θ A' A B' B
+  , inst_expr Θ A' A
+  → (forall x, x `notin` L → inst_expr Θ (B' ^`′ x) (B ^` x))
+  → inst_expr Θ (ae_pi A' B') (e_pi A B)
+| inst_all : forall L Θ A' A B' B
+  , inst_expr Θ A' A
+  → (forall x, x `notin` L → inst_expr Θ (B' ^`′ x) (B ^` x))
+  → inst_expr Θ (ae_all A' B') (e_all A B)
+where "T ⊩ e1 ⇝ e2" := (inst_expr T e1 e2) : type_scope
+.
+
+Lemma inst_e_wf_ss : forall Θ e' e,
+  Θ ⊩ e' ⇝ e → wf_ss Θ.
+Proof with induction 1; auto.
+  idtac...
+Qed.
+
+Require Import Program.Tactics.
+
+Scheme lc_ae_body_mut := Induction for lc_aexpr Sort Prop
+  with lc_body_ae_mut := Induction for lc_abody Sort Prop.
+
+Hint Extern 2 =>
+  match goal with
+  | |- context [open_body_wrt_expr _ _] =>
+    unfold open_body_wrt_expr; simpl
+  | |- context [open_abody_wrt_aexpr _ _] =>
+    unfold open_abody_wrt_aexpr; simpl
+end : lc
+.
+
+Hint Resolve lc_ae_abs_exists : lc.
+Hint Resolve lc_ae_bind_exists : lc.
+Hint Resolve lc_e_abs_exists : lc.
+Hint Resolve lc_e_bind_exists : lc.
+
+Lemma inst_ae_lc : forall Θ e' e,
+  Θ ⊩ e' ⇝ e → lc_aexpr e'.
+Proof.
+  induction 1;
+    solve [auto | pick fresh x; eauto 6 with lc].
+Qed.
+
+
+Lemma inst_e_lc : forall Θ e' e,
+    Θ ⊩ e' ⇝ e → lc_expr e.
+Proof.
+  induction 1; try solve [auto | pick fresh x; eauto 6 with lc].
+Admitted.
+
+
+#[export]
+Hint Resolve inst_e_wf_ss : core.
+
+Reserved Notation "T ⊩ ob ⇝? dob" (at level 65, ob at level 58, no associativity).
+Inductive inst_obind : subst_set → obind → obindd → Prop :=
+| instob_none : forall Θ, inst_obind Θ ob_none dob_none
+| instob_bind : forall Θ x A' A, inst_obind Θ (x :?′ A') (x :? A)
+where "T ⊩ ob ⇝? dob" := (inst_obind T ob dob) : type_scope
+.
+
+Reserved Notation "T ⊩ w1 ⇝′ w2" (at level 65, w1 at level 58).
+Reserved Notation "T1 ⊩ G1 ⟿ G2 ⫣ T2" (at level 65, G1 at level 58, G2 at level 58).
+Inductive inst_work : subst_set → work → dwork → Prop :=
+| instw_check : forall Θ ob ob' e1 e1' e2 e2' A A'
+  , inst_obind Θ ob' ob → inst_expr Θ A' A
+  → inst_expr Θ e1' e1 → inst_expr Θ e2' e2
+  → inst_work Θ (ob' ⊢? e1' <: e2' ⇐′ A') (ob ⊢? e1 <: e2 ⇐ A)
+| instw_cpct  : forall Θ A A' B B'
+  , inst_expr Θ A' A → inst_expr Θ B' B
+  → inst_work Θ (A' ≲′ B') (A ≲ B)
+| instw_infer : forall L Θ Θ' e1 e1' e2 e2' c c'
+  , inst_expr Θ e1' e1 → inst_expr Θ e2' e2
+  → (forall x, x `notin` L → inst_wl Θ (c' $′ `′x) (c $ `x) Θ')
+  → inst_work Θ (e1' <: e2' ⇒′ c') (e1 <: e2 ⇒ c)
+| instw_iapp : forall L Θ Θ' A A' e e1' e2' c c'
+  , inst_expr Θ e1' e → inst_expr Θ e2' e
+  → (forall x, x `notin` L → inst_wl Θ (c' $′ `′x) (c $ `x) Θ')
+  → inst_work Θ (A' ⋅ e1' & e2' ⇒′ c') (A ⋅ e ⇒ c)
+| instw_red : forall L Θ Θ' A A' c c'
+  , inst_expr Θ A' A
+  → (forall x, x `notin` L → inst_wl Θ (c' $′ `′x) (c $ `x) Θ')
+  → inst_work Θ (A' ⟼′ c') (A ⟼ c)
+where "T ⊩ w1 ⇝′ w2" := (inst_work T w1 w2) : type_scope
+with inst_wl  : subst_set → worklist → dworklist → subst_set → Prop :=
+| instwl_nil  : forall Θ, inst_wl Θ wl_nil dwl_nil Θ
+| instwl_cons : forall Θ Θ' Γ Γ' w w'
+  , inst_wl Θ Γ' Γ Θ' → inst_work Θ' w' w
+  → inst_wl Θ (Γ' ⊨′ w') (Γ ⊨ w) Θ'
+| instwl_var  : forall Θ Θ' Γ Γ' x A A'
+  , inst_wl Θ Γ' Γ Θ' → x `notin` dom Θ → inst_expr Θ' A' A
+  → inst_wl Θ (Γ' ,′ x :′ A') (Γ ,' x : A) (Θ'; x : A!)
+| instwl_kv : forall Θ Θ' Γ Γ' x k
+  , inst_wl Θ Γ' Γ Θ' → x `notin` dom Θ
+  → inst_wl Θ (Γ' ,′ ⧼^x⧽) Γ (Θ'; x ≔ ⧼k⧽)
+| instwl_ex : forall Θ Θ' Γ Γ' x A' A e
+  , mono_type e
+  → inst_wl Θ Γ' Γ Θ' → x `notin` dom Θ → inst_expr Θ' A' A
+  → inst_wl Θ (Γ' ,′ ^x :′ A') Γ (Θ'; x : A ≔ e)
+where "T1 ⊩ G1 ⟿ G2 ⫣ T2" := (inst_wl T1 G1 G2 T2) : type_scope
+.
+
+#[export]
+Hint Constructors inst_expr inst_obind inst_work inst_wl : core.
+
+
+Definition transfer' (Γ' : worklist) (Γ : dworklist) : Prop :=
+  exists Θ, inst_wl nil Γ' Γ Θ.
+
+Hint Extern 2 (_ = _) => simpl; congruence : core.
+
+Lemma inst_e_det : forall e' Θ e1 e2,
+  uniq Θ → Θ ⊩ e' ⇝ e1 → Θ ⊩ e' ⇝ e2 → e1 = e2.
+Proof.
+Admitted.
+
+
+
+Lemma inst_wl_split : forall Γ1' Γ2' Γ Θ Θ'
+  , Θ ⊩ Γ1' ⫢′ Γ2' ⟿ Γ ⫣ Θ'
+  → exists Γ1 Γ2 Θ0
+    , Γ = Γ1 ⫢ Γ2
+    ∧ Θ  ⊩ Γ1' ⟿ Γ1 ⫣ Θ0
+    ∧ Θ0 ⊩ Γ2' ⟿ Γ2 ⫣ Θ'.
+Proof.
+  induction Γ2'; simpl; intros.
+  - exists Γ, dwl_nil, Θ'; simpl; solve [auto].
+  - inversion H; subst.
+    pose proof (IHΓ2' _ _ _ H3) as (Γ1 & Γ2 & Θ0 & E & Inst1 & Inst2).
+    exists Γ1, (Γ2 ⊨ w0), Θ0. auto.
+  - destruct b.
+    + inversion H; subst.
+      pose proof (IHΓ2' _ _ _ H4) as (Γ1 & Γ2 & Θ0 & E & Inst1 & Inst2).
+      exists Γ1, (Γ2 ,' x : A0), Θ0. admit.
+    + inversion H; subst.
+      pose proof (IHΓ2' _ _ _ H5) as (Γ1 & Γ2 & Θ0 & E & Inst1 & Inst2).
+      exists Γ1, Γ2, Θ0. admit.
+    + inversion H; subst.
+      pose proof (IHΓ2' _ _ _ H3) as (Γ1 & Γ2 & Θ0 & E & Inst1 & Inst2).
+      exists Γ1, Γ2, Θ0. admit.
+Admitted.
+
+Scheme wl_mut   := Induction for worklist Sort Prop
+  with work_mut := Induction for work     Sort Prop.
+
+Scheme wins_mut   := Induction for inst_work Sort Prop
+  with wlinst_mut := Induction for inst_wl   Sort Prop.
+
+Lemma inst_wl_ss_expand : forall Θ Γ' Γ Θ'
+  , Θ ⊩ Γ' ⟿ Γ ⫣ Θ'
+  → exists Θ0, Θ ;; Θ0 = Θ'.
+Proof.
+  induction 1; try pose proof IHinst_wl as (Θ0 & <-).
+  - now exists nil.
+  - assumption.
+  - now exists (Θ0; x : A !).
+  - now exists (Θ0; x ≔ ⧼k⧽).
+  - now exists (Θ0; x : A ≔ e).
+Qed.
+
+Lemma inst_e_weakening : forall Θ e' e Θ',
+  Θ ⊩ e' ⇝ e → Θ ;; Θ' ⊩ e' ⇝ e.
+Proof.
+  induction 1; eauto.
+Admitted.
+
+#[local]
+Hint Resolve inst_e_weakening : inst_weakening.
+
+Lemma inst_ob_weakening : forall Θ Θ' ob' ob,
+  Θ ⊩ ob' ⇝? ob → Θ ;; Θ' ⊩ ob' ⇝? ob.
+Proof.
+  induction 1; eauto.
+Qed.
+
+#[local]
+Hint Resolve inst_ob_weakening : inst_weakening.
+
+(* doable *)
+Lemma inst_w_weakening : forall Θ w' w Θ',
+  Θ ⊩ w' ⇝′ w → Θ ;; Θ' ⊩ w' ⇝′ w.
+Proof.
+  intros.
+  pattern Θ, w', w, H.
+  apply wins_mut with
+      (P0 := fun Θ Γ' Γ Θ1 (_ : Θ ⊩ Γ' ⟿ Γ ⫣ Θ1) =>
+               forall Θ0, Θ1 = Θ ;; Θ0 → Θ ⊩ Γ' ⟿ Γ ⫣ Θ ;; Θ0 → Θ ;; Θ' ⊩ Γ' ⟿ Γ ⫣ Θ ;; Θ' ;; Θ0);
+    intros.
+Admitted.
+
+Lemma inst_e_rev_subst : forall v' v x e' e0 Θ
+  , Θ ⊩ [v' /′ x] e' ⇝ e0 → Θ ⊩ v' ⇝ v
+  → exists e, [v /' x] e = e0 ∧ Θ ⊩ e' ⇝ e.
+Proof.
+  intros * H.
+  assert (lc_aexpr e') by admit.
+  generalize dependent e0. generalize dependent Θ.
+  induction H0; simpl; intros.
+  - exists (` x0). simpl. destruct (x0 == x).
+    + admit.
+    + admit.
+  - admit.
+  - admit.
+  - admit.
+  - admit.
+  - admit.
+  - admit.
+  - admit.
+  - admit.
+Admitted.
+
+Lemma inst_wl_rev_subst : forall Γ' x e' e Γ0 Θ Θ'
+  , Θ ⊩ subst_worklist e' x Γ' ⟿ Γ0 ⫣ Θ'
+  → Θ ⊩ e' ⇝ e
+  → exists Γ
+    , subst_dworklist e x Γ = Γ0
+    ∧ Θ ⊩ Γ' ⟿ Γ ⫣ Θ'.
+Proof.
+  intro Γ'.
+  pattern Γ'.
+  apply wl_mut with
+    (P0 := fun w' =>
+      forall x e' e w0 Θ
+      , Θ ⊩ subst_work e' x w' ⇝′ w0
+        → Θ ⊩ e' ⇝ e
+        → exists w, subst_dwork e x w = w0 ∧ Θ ⊩ w' ⇝′ w); simpl; intros.
+  - inversion H; subst.
+    exists dwl_nil; simpl; repeat split; auto.
+  - simpl in H1. inversion H1; subst. admit.
+  - destruct b; inversion H0; subst; simpl in *; admit.
+  - admit.
+  -
+Admitted.
