src-lite/simplified_ind.v
@@ -1,0 +1,63 @@
+Require Export decl_notations.
+
+Lemma lc_body_e : forall e A,
+    lc_body (b_anno e A) -> lc_expr e.
+Proof.
+  now inversion 1.
+Qed.
+
+Lemma lc_body_b : forall e A,
+    lc_body (b_anno e A) -> lc_expr A.
+Proof.
+  now inversion 1.
+Qed.
+
+#[local]
+Hint Resolve lc_body_b lc_body_e : core.
+
+#[local]
+Hint Unfold open_body_wrt_expr : core.
+
+Lemma lc_expr_ind' : ∀ (P : expr → Prop)
+  , (∀ (x : var), P (e_var_f x))
+  → (∀ (k : kind), P ⧼ k ⧽)
+  → (∀ (n : number), P (e_num n))
+  → P e_int
+  → (∀ (A : expr), lc_expr A → P A → P (e_bot A))
+  → (∀ (e1 e2 : expr)
+    , lc_expr e1 → P e1 → lc_expr e2 → P e2 → P (e_app e1 e2))
+  → (∀ (A e B : expr)
+    , lc_expr A → P A
+    → (∀ (x : exprvar), lc_expr (e ^` x))
+    → (forall (x : exprvar), lc_expr (B ^` x))
+    → P (λ_ A, e : B))
+  → (∀ (A B : expr)
+    , lc_expr A → P A → (∀ (x : exprvar), lc_expr (B ^` x))
+    → (∀ (x : exprvar), P (B ^` x)) → P (e_pi A B))
+  → (∀ (A e B : expr)
+    , lc_expr A → P A
+    → (∀ x, lc_expr (e ^` x))
+    → (forall x, lc_expr (B ^` x))
+    → P (Λ A, e : B))
+  → (∀ (A B : expr)
+    , lc_expr A → P A → (∀ (x : exprvar), lc_expr (B ^` x))
+    → (∀ (x : exprvar), P (B ^` x)) → P (e_all A B))
+  → (∀ (A e : expr)
+    , lc_expr A → P A → lc_expr e → P e → P (e_castup A e))
+  → (∀ (e : expr), lc_expr e → P e → P (e_castdn e))
+  → ∀ (e : expr), lc_expr e → P e.
+Proof.
+  intros.
+  match goal with
+  | H : lc_expr ?e |- ?P ?e =>
+    induction H;
+    (* solve all cases except for special ones with 'body' *)
+    eauto; repeat
+    match goal with
+    | H : context [open_body_wrt_expr ?b _] |- _ =>
+      destruct b; unfold open_body_wrt_expr in H; simpl in H
+    end;
+    eauto
+  end
+.
+Qed.
