src-lite/wl_properties.v
@@ -1,0 +1,16 @@
+Require Import worklist.
+Require Import decl_worklist.
+Require Import wl_transfer.
+
+Theorem wl_sound : forall Γ',
+    ⪧′ Γ' → exists Γ, Γ' ⟿ Γ ∧ ⪧ Γ.
+Proof.
+  intros * H.
+  induction H; intros.
+  (* nil *)
+  - eauto.
+  (* var *)
+  - admit.
+  (* num *)
+  - admit.
+Admitted.
